Begin fixing flat_pattern for eval, big issue
The problem is that the order of execution of source declarations
and the order the compiler sees them in is now totally different
with eval, so source-level semantic side-conditions (e.g. that no
type can be re-declared) don't give compiler guarantees.

compiler/backend/proofs/flat_patternProofScript.sml
@@ -627,7 +627,9 @@ QED
 val s = ``s:('c, 'ffi) flatSem$state``;
 val s1 = mk_var ("s1", type_of s);
 val s2 = mk_var ("s2", type_of s);
-val t = mk_var ("t", type_of s);
+(* on the right side of the state relation, the pattern compiler's config is
+   also needed in the compiler state *)
+val t = ``t:((config # 'c), 'ffi) flatSem$state``;
 
 Definition prev_cfg_rel_def:
   prev_cfg_rel past_cfg cur_cfg =
@@ -691,7 +693,7 @@ Definition state_rel_def:
 End
 
 Theorem state_rel_initial_state:
-  state_rel cfg (initial_state ffi k T ec) (initial_state ffi k T ec)
+  state_rel cfg (initial_state ffi k T ec) (initial_state ffi k T ec')
 Proof
   fs [state_rel_def, initial_state_def]
 QED
@@ -1141,14 +1143,21 @@ QED
 
 Definition c_type_map_rel_def:
   c_type_map_rel c type_map = (!stmp ty_id len.
-    (((stmp, SOME ty_id), len) ∈ c) <=>
+    (((stmp, SOME ty_id), len) ∈ c) ==>
         ?tys. lookup ty_id type_map = SOME tys /\ MEM (stmp, len) tys)
 End
 
-Theorem ctor_same_type_v_cons_is_sibling_subspt:
+Theorem c_type_map_rel_subspt:
+  c_type_map_rel c tm /\ subspt tm tm' ==>
+  c_type_map_rel c tm'
+Proof
+  fs [c_type_map_rel_def, subspt_lookup]
+  \\ metis_tac []
+QED
+
+Theorem ctor_same_type_v_cons_is_sibling:
   ctor_same_type (SOME stmp) (SOME stmp') /\
-  c_type_map_rel c tm' /\
-  subspt tm tm' /\
+  c_type_map_rel c tm /\
   (stmp, len) ∈ c /\
   (stmp', len') ∈ c /\
   stmp' = (x, SOME y) ==>
@@ -1157,14 +1166,22 @@ Proof
   simp [c_type_map_rel_def]
   \\ Cases_on `stmp` \\ Cases_on `stmp'` \\ rw []
   \\ rfs [ctor_same_type_def]
+  \\ first_x_assum (fn t => drule t \\ imp_res_tac t)
   \\ rveq \\ fs []
   \\ rveq \\ fs []
   \\ simp [pattern_semanticsTheory.is_sibling_def]
-  \\ fs [subspt_lookup]
-  \\ Cases_on `lookup y tm` \\ simp [pattern_semanticsTheory.is_sibling_def]
-  \\ first_x_assum drule
-  \\ rw []
-  \\ simp []
+QED
+
+Theorem is_sibling_lookup_subspt:
+  pattern_semantics$is_sibling (x, len) (lookup y tm) /\
+  subspt tm' tm ==>
+  pattern_semantics$is_sibling (x, len) (lookup y tm')
+Proof
+  rw [subspt_lookup]
+  \\ first_x_assum (qspec_then `y` mp_tac)
+  \\ Cases_on `lookup y tm` \\ Cases_on `lookup y tm'`
+  \\ fs [pattern_semanticsTheory.is_sibling_def]
+  \\ rw [] \\ simp []
 QED
 
 Theorem encode_pat_match_simulation:
@@ -1205,10 +1222,14 @@ Proof
     \\ fs [pmatch_stamps_ok_OPTREL, v_cons_in_c_def, OPTREL_def]
     \\ rfs [] \\ fs []
     \\ simp [pmatch_def]
-    \\ drule_then drule ctor_same_type_v_cons_is_sibling_subspt
+    \\ drule_then drule ctor_same_type_v_cons_is_sibling
     \\ rpt (disch_then drule)
-    \\ rpt (CASE_TAC \\ fs [ctor_same_type_def, same_ctor_def, pmatch_def,
-            pattern_semanticsTheory.is_sibling_def])
+    \\ every_case_tac \\ fs [ctor_same_type_def, same_ctor_def, pmatch_def,
+            pattern_semanticsTheory.is_sibling_def]
+    \\ rveq \\ fs []
+    \\ rpt strip_tac
+    \\ drule_then drule is_sibling_lookup_subspt
+    \\ simp []
   )
   >- (
     (* refs *)
@@ -1580,6 +1601,12 @@ Proof
   simp [state_rel_def, dec_clock_def]
 QED
 
+Theorem cfg_inv_dec_clock:
+  cfg_inv cfg (dec_clock s) = cfg_inv cfg s
+Proof
+  simp [dec_clock_def, cfg_inv_def]
+QED
+
 Theorem OPTION_ALL_FORALL:
   OPTION_ALL P x = (!y. x = SOME y ==> P y)
 Proof
@@ -1623,11 +1650,112 @@ Definition cfg_inv_def:
   c_type_map_rel s.c cfg.type_map
 End
 
-(* FIXME: cheated do_eval, and for a stateful phase, the oracle
-   nonsense will probaby be tricky *)
+Theorem cfg_inv_prev_cfg_rel:
+  cfg_inv cfg s /\ prev_cfg_rel cfg cfg' /\
+  ¬MEM [] (toList cfg'.type_map) ==>
+  cfg_inv cfg' s
+Proof
+  rw [cfg_inv_def, prev_cfg_rel_def] \\ fs []
+  \\ metis_tac [c_type_map_rel_subspt]
+QED
+
+Theorem s_rel_eval:
+  state_rel cfg s t ==>
+  ?c st st'. s.eval_mode = Eval <| compile := c; compiler_state := st' |> /\
+    t.eval_mode = Eval <| compile := (\env (st, st') decs.
+        let (decs, env, st') = c env st' decs in
+        let (st, decs) = compile_decs st decs in
+        (decs, env, (st, st'))); compiler_state := (st, st') |> /\
+    prev_cfg_rel cfg st /\ ~ MEM [] (toList st.type_map)
+Proof
+  cheat
+QED
+
+Theorem v_to_environment_rel:
+  v_to_environment envv = SOME env /\ v_rel cfg envv envv' ==>
+  v_to_environment envv' = SOME env
+Proof
+  cheat
+QED
+
+Theorem v_to_decs_rel:
+  v_to_decs decsv = SOME decs /\ v_rel cfg decsv decsv' ==>
+  v_to_decs decsv' = SOME decs
+Proof
+  cheat
+QED
+
+Theorem environment_to_v_rel:
+  v_rel cfg (environment_to_v env) (environment_to_v env)
+Proof
+  cheat
+QED
+
+(* it's not possible to relate cfg-s to states.
+   jumping between closures often means jumping between states the compiler
+   was in, but the compiler is always in the future, having at least compiled
+   the code the closure came from.
+   in (eval c; z) the compiler sees z first, but the decs from c are the first
+   to be executed.
+
+   we can derive a failure here, with
+   (eval (c -> (eval (c -> Dtype 12)); x)) ; fail; Dtype 12).
+   The compiler sees the declaration of type 12 from the last dec when it is
+   compiling x, although it is not yet in scope, but the declaration from the
+   doubly-nested eval is.
+
+   The only obvious alternative is a painful syntactic property.
+*)
+
+Theorem do_eval_thm:
+  do_eval (REVERSE xs) s = SOME (decs, s', rv) /\
+  state_rel cfg s t /\
+  cfg_inv cfg t /\
+  LIST_REL (v_rel cfg) xs ys ==>
+  ?rv' cfg' decs' t'.
+  do_eval (REVERSE ys) t = SOME (decs', t', rv') /\
+  state_rel cfg s' t' /\
+  cfg_inv cfg t' /\
+  cfg_inv cfg' t' /\
+  v_rel cfg rv rv' /\
+  decs' = SND (compile_decs cfg' decs) /\
+  t'.c = t.c /\
+  prev_cfg_rel cfg cfg'
+Proof
+  rw []
+  \\ imp_res_tac s_rel_eval
+  \\ fs [do_eval_def, case_eq_thms]
+  \\ fs [Q.SPECL [`xs`, `[y1; y2]`] listTheory.SWAP_REVERSE_SYM]
+  \\ rpt (pairarg_tac \\ fs [])
+  \\ rveq \\ fs []
+  \\ rveq \\ fs []
+  \\ drule_then drule v_to_environment_rel
+  \\ drule_then drule v_to_decs_rel
+  \\ rw []
+  \\ rpt (pairarg_tac \\ fs [])
+  \\ rveq \\ fs []
+  \\ qexists_tac `st`
+  \\ simp [environment_to_v_rel]
+  \\ drule_then drule cfg_inv_prev_cfg_rel
+  \\ fs [cfg_inv_def]
+  \\ fs [state_rel_def]
+QED
+
+Theorem EVERY_v_cons_in_c_SUBSET:
+  !vs. EVERY (v_cons_in_c c) vs /\ c ⊆ c' ==> EVERY (v_cons_in_c c') vs
+Proof
+  simp [EVERY_MEM] \\ metis_tac [v_cons_in_c_SUBSET]
+QED
+
+Theorem EVERY_v_cons_in_c_o_SUBSET = EVERY_v_cons_in_c_SUBSET
+    |> Q.SPEC `MAP f xs`
+    |> REWRITE_RULE [EVERY_MAP, GSYM o_DEF]
+
+(* s/t swapped around in this file *)
 
 Theorem compile_exps_evaluate:
-  (!env1 ^s1 xs t1 r1 i sg ys N env2 ^s2 cfg prev_cfg.
+
+  (!env1 ^s1 xs t1 r1 i sg ys N env2 s2 cfg prev_cfg.
     evaluate env1 s1 xs = (t1, r1) /\
     compile_exps prev_cfg xs = (i, sg, ys) /\
     r1 <> Rerr (Rabort Rtype_error) /\
@@ -1640,8 +1768,8 @@ Theorem compile_exps_evaluate:
       result_rel (LIST_REL (v_rel cfg)) (v_rel cfg) r1 r2 /\
       state_rel cfg t1 t2 /\
       evaluate env2 s2 ys = (t2, r2) /\
-      EVERY (v_cons_in_c s2.c) (result_vs r2) /\
-      t2.c = s2.c /\
+      EVERY (v_cons_in_c t2.c) (result_vs r2) /\
+      s2.c ⊆ t2.c /\
       cfg_inv cfg t2
   ) /\
   (!^s1 dec t1 res cfg cfg' dec' s2.
@@ -1668,12 +1796,15 @@ Theorem compile_exps_evaluate:
   ?t2 res'.
   evaluate_decs s2 decs' = (t2, res') /\
   OPTREL (exc_rel (K (K T))) res res' /\
+  s2.c ⊆ t2.c /\
   t1.ffi = t2.ffi /\
   (res = NONE ==>
     state_rel cfg' t1 t2 /\ cfg_inv cfg' t2 /\
     prev_cfg_rel cfg cfg')
   )
+
 Proof
+
   ho_match_mp_tac evaluate_ind
   \\ simp [evaluate_def, compile_exps_def, result_vs_def]
   \\ rpt (gen_tac ORELSE disch_tac ORELSE conj_tac)
@@ -1698,10 +1829,12 @@ Proof
     \\ rveq \\ fs []
     \\ fs [case_eq_thms, pair_case_eq] \\ rveq \\ fs [] \\ rveq \\ fs []
     \\ imp_res_tac evaluate_length
+    \\ drule_then drule EVERY_v_cons_in_c_o_SUBSET
     \\ rpt (first_x_assum drule \\ rw [])
     \\ fs [quantHeuristicsTheory.LIST_LENGTH_2, listTheory.LENGTH_CONS]
     \\ rveq \\ fs []
     \\ rveq \\ fs []
+    \\ metis_tac [v_cons_in_c_SUBSET, SUBSET_TRANS]
   )
   >- (
     rpt (first_x_assum drule \\ rw [])
@@ -1711,7 +1844,6 @@ Proof
     \\ imp_res_tac evaluate_length
     \\ rpt (first_x_assum drule \\ rw [])
     \\ fs [quantHeuristicsTheory.LIST_LENGTH_2, listTheory.LENGTH_CONS]
-    \\ rveq \\ fs []
     \\ rveq \\ fs []
   )
   >- (
@@ -1747,11 +1879,12 @@ Proof
     \\ drule_then drule evaluate_compile_pat_rhs
     \\ simp [LESS_MAX_ADD]
     \\ rpt (disch_then drule)
+    \\ drule_then drule EVERY_v_cons_in_c_o_SUBSET
     \\ simp []
-    \\ disch_tac
+    \\ rpt disch_tac
     \\ fs []
     \\ last_x_assum (drule_then (drule_then drule))
-    \\ simp [LESS_MAX_ADD]
+    \\ fs [LESS_MAX_ADD, SUBSET_DEF]
   )
   >- (
     (* Conv, no tag *)
@@ -1772,7 +1905,7 @@ Proof
     \\ simp [PULL_EXISTS, v_rel_rules, EVERY_REVERSE]
     \\ imp_res_tac evaluate_length
     \\ fs [state_rel_def]
-    \\ rfs []
+    \\ rfs [SUBSET_DEF]
   )
   >- (
     drule_then drule env_rel_ALOOKUP
@@ -1794,13 +1927,16 @@ Proof
     \\ fs [env_rel_def]
     \\ metis_tac [FST, SND, HD, prev_cfg_rel_refl]
   )
+
   >- (
     (* App *)
+
     last_x_assum (drule_then (drule_then drule))
     \\ rw []
     \\ fs [case_eq_thms] \\ rveq \\ fs [] \\ rveq \\ fs []
     \\ Cases_on `op = Opapp`
     >- (
+
       fs [option_case_eq, pair_case_eq]
       \\ rveq \\ fs []
       \\ drule_then drule do_opapp_thm_REVERSE
@@ -1811,18 +1947,49 @@ Proof
       \\ fs [Q.ISPEC `(a, b)` EQ_SYM_EQ]
       \\ imp_res_tac state_rel_dec_clock
       \\ last_x_assum (first_assum o mp_then (Pat `state_rel _ _ _`) mp_tac)
+      \\ simp [cfg_inv_dec_clock]
       \\ simp [dec_clock_def]
-      \\ disch_then irule
-      \\ drule do_opapp_v_inv
-      \\ rfs [cfg_inv_def]
-      \\ rw [EVERY_REVERSE]
-      \\ simp [env_rel_def]
-      \\ metis_tac [LE_LT1, LESS_EQ_REFL]
+      \\ disch_then drule
+      \\ disch_then (qspecl_then [`i' + 1`, `<|v := nvs2|>`] mp_tac)
+      \\ impl_tac
+      >- (
+        simp [env_rel_def]
+        \\ metis_tac [do_opapp_v_inv, EVERY_REVERSE]
+      )
+      \\ rw []
+      \\ fs [SUBSET_DEF]
     )
     \\ Cases_on `op = Eval`
     >- (
-      fs []
-      \\ cheat
+
+      fs [option_case_eq, pair_case_eq]
+      \\ rveq \\ fs []
+      \\ drule_then drule do_eval_thm
+      \\ rpt (disch_then drule)
+      \\ strip_tac \\ fs []
+      \\ imp_res_tac state_rel_IMP_clock
+      \\ fs [bool_case_eq, Q.ISPEC `(a, b)` EQ_SYM_EQ]
+      \\ fs [pair_case_eq]
+      \\ rename [`_ = SND (compile_decs cfg' decs2)`]
+      \\ Cases_on `compile_decs cfg' decs2`
+      \\ fs []
+      \\ imp_res_tac state_rel_dec_clock
+
+      \\ last_x_assum drule
+      \\ imp_res_tac state_rel_next_cfg
+      \\ disch_then (first_assum o mp_then (Pat `state_rel _ _ _`) mp_tac)
+      \\ impl_tac
+      >- (
+        simp [cfg_inv_dec_clock] \\ CCONTR_TAC \\ fs []
+      )
+      \\ rw []
+      \\ fs [option_case_eq] \\ rveq \\ fs []
+      \\ fs [OPTREL_def]
+      \\ simp [PULL_EXISTS]
+
+      \\ TRY (fs [state_rel_def]
+
+      \\ fs []
     )
     \\ fs [option_case_eq, pair_case_eq]
     \\ rveq \\ fs []
@@ -1953,6 +2120,8 @@ Proof
     \\ rveq \\ fs []
     \\ simp [OPTREL_def]
   )
+
+
   >- (
     rename [`compile_dec cfg (Dtype id ctors)`]
     \\ imp_res_tac state_rel_IMP_check_ctor
